A12Kernel.lean
@@ -85,6 +85,7 @@ import A12Kernel.Elaboration.ValueAsDateTimeComponents
 import A12Kernel.Elaboration.ValueAsDateTimeWorldComponents
 import A12Kernel.Elaboration.ConstructedDateComponents
 import A12Kernel.Elaboration.ConstructedDateEvaluation
+import A12Kernel.Elaboration.ConstructedDateShiftEvaluation
 import A12Kernel.Elaboration.TemporalComputationResult
 import A12Kernel.Elaboration.FullDateComputationApplication
 import A12Kernel.Elaboration.DateTimeComputationApplication
